

## Part (2) — Analytic Geometry Proof (Short, copy into ipynb)

**Goal:** Prove

$$BE \cdot DH = BD \cdot EH.$$

---

### 1) Coordinate setup

Let  $C = (0, 0)$  -  $B = (-1, 0)$  -  $D = (0, 1)$

Then  $\angle C = 90^\circ$  and  $BC = CD = 1$ . Since  $AD \parallel BC$ , line  $AD$  is horizontal, so  $A = (a, 1)$ .

Let  $E \in CD \Rightarrow E = (0, t)$ , where  $0 < t < 1$ . Given  $DE = AD$ :  $-DE = 1 - t - AD = |a|$

So  $|a| = 1 - t$ . From the diagram  $A$  is left of  $D$ , hence  $a = -(1 - t) = t - 1$ . Therefore

$$A = (t - 1, 1), \quad E = (0, t).$$

---

### 2) Lines $BD$ and $EF$

Line  $BD$  through  $(-1, 0)$  and  $(0, 1)$ :

$$BD : y = x + 1.$$

Slope of  $AB$ :

$$m_{AB} = \frac{1 - 0}{(t - 1) - (-1)} = \frac{1}{t}.$$

So  $EF \perp AB$  has slope  $-t$ , and since it passes through  $E = (0, t)$ :

$$EF : y = t - tx.$$

---

### 3) Intersection $H = BD \cap EF$

Solve

$$x + 1 = t - tx \Rightarrow x = \frac{t - 1}{t + 1}, \quad y = x + 1 = \frac{2t}{t + 1}.$$

So

$$H = \left( \frac{t-1}{t+1}, \frac{2t}{t+1} \right).$$


---

#### 4) Distances via a common scale factor

Compute vectors:

$$H - D = \left( \frac{t-1}{t+1}, \frac{t-1}{t+1} \right) = \frac{t-1}{t+1}(1, 1),$$

$$H - E = \left( \frac{t-1}{t+1}, \frac{2t}{t+1} - t \right) = \left( \frac{t-1}{t+1}, -\frac{t(t-1)}{t+1} \right) = \frac{t-1}{t+1}(1, -t).$$

Hence

$$DH = \frac{1-t}{t+1} \|(1, 1)\| = \frac{1-t}{t+1} \sqrt{2}, \quad EH = \frac{1-t}{t+1} \|(1, -t)\| = \frac{1-t}{t+1} \sqrt{1+t^2}.$$

Also

$$BD = \|(1, 1)\| = \sqrt{2}, \quad BE = \|(1, t)\| = \sqrt{1+t^2}.$$


---

#### 5) Finish

$$BE \cdot DH = \sqrt{1+t^2} \cdot \frac{1-t}{t+1} \sqrt{2} = \sqrt{2} \cdot \frac{1-t}{t+1} \sqrt{1+t^2} = BD \cdot EH.$$

✓ Proven.